backends/lean/Aeneas/Std/String.lean
@@ -3,6 +3,8 @@ import Aeneas.Std.Slice
 
 namespace Aeneas.Std
 
+open Result
+
 def Str := Slice U8
 
 /-- TODO: we shouldn't use `decide +native` but it seems we can't reduce it otherwise. -/
@@ -16,5 +18,16 @@ def toStr (s : String) (h : s.toByteArray.size ≤ U32.max := by decide +native)
       sorry ⟩
 
 example : Str := toStr "hello"
+
+/-- `str::to_owned` via `ToOwned<String> for str`. Takes a `Str` (modeled as
+`Slice U8`) and returns an owned `String`.
+
+- Docs: https://doc.rust-lang.org/core/borrow/trait.ToOwned.html#tymethod.to_owned
+- Source: https://github.com/rust-lang/rust/blob/1.85.0/library/alloc/src/str.rs
+-/
+@[rust_fun "alloc::str::{alloc::borrow::ToOwned<str, alloc::string::String>}::to_owned"]
+def Str.Insts.AllocBorrowToOwnedString.to_owned (s : Str) : Result String :=
+  ok (String.fromUTF8!
+    ⟨ (s.val.map (fun x => (UInt8.ofNat x.val))).toArray ⟩)
 
 end Aeneas.Std
